zoo/iris/base_logic/lib: Generalize ghost_var.

theories/zoo/iris/base_logic/lib/ghost_var.v
@@ -10,30 +10,40 @@ From zoo.iris Require Import
 From zoo Require Import
   options.
 
-Class GhostVarG Σ A := {
-  #[local] ghost_var_G_inG :: inG Σ (dfrac_agreeR $ leibnizO A) ;
+Class GhostVarG Σ F := {
+  #[local] ghost_var_G_inG :: inG Σ (dfrac_agreeR $ oFunctor_apply F $ iPropO Σ) ;
 }.
 
-Definition ghost_var_Σ A := #[
-  GFunctor (dfrac_agreeR $ leibnizO A)
+Definition ghost_var_Σ F `{!oFunctorContractive F} := #[
+  GFunctor (dfrac_agreeRF F)
 ].
-#[global] Instance subG_ghost_var_Σ Σ A :
-  subG (ghost_var_Σ A) Σ →
-  GhostVarG Σ A.
+#[global] Instance subG_ghost_var_Σ Σ F `{!oFunctorContractive F} :
+  subG (ghost_var_Σ F) Σ →
+  GhostVarG Σ F.
 Proof.
   solve_inG.
 Qed.
 
 Section ghost_var_G.
-  Context `{ghost_var_G : !GhostVarG Σ A}.
-
-  Implicit Types a : A.
+  Context `{ghost_var_G : !GhostVarG Σ F}.
 
   Definition ghost_var γ dq a :=
-    own γ (to_dfrac_agree (A := leibnizO A) dq a).
+    own γ (to_dfrac_agree dq a).
 
-  #[global] Instance ghost_var_timeless γ q a :
-    Timeless (ghost_var γ q a).
+  #[global] Instance ghost_var_nonexpansive γ dq :
+    NonExpansive (ghost_var γ dq).
+  Proof.
+    solve_proper.
+  Qed.
+  #[global] Instance ghost_var_proper γ dq :
+    Proper ((≡) ==> (≡)) (ghost_var γ dq).
+  Proof.
+    solve_proper.
+  Qed.
+
+  #[global] Instance ghost_var_timeless γ dq a :
+    Discrete a →
+    Timeless (ghost_var γ dq a).
   Proof.
     apply _.
   Qed.
@@ -46,7 +56,8 @@ Section ghost_var_G.
   #[global] Instance ghost_var_fractional γ a :
     Fractional (λ q, ghost_var γ (DfracOwn q) a).
   Proof.
-    intros q1 q2. rewrite -own_op -frac_agree_op //.
+    intros q1 q2.
+    rewrite -own_op -frac_agree_op //.
   Qed.
   #[global] Instance ghost_var_as_fractional γ a q :
     AsFractional (ghost_var γ (DfracOwn q) a) (λ q, ghost_var γ (DfracOwn q) a) q.
@@ -61,40 +72,48 @@ Section ghost_var_G.
   Proof.
     apply own_alloc. done.
   Qed.
+  Lemma ghost_var_alloc_cofinite (γs : gset gname) a :
+    ⊢ |==>
+      ∃ γ,
+      ⌜γ ∉ γs⌝ ∗
+      ghost_var γ (DfracOwn 1) a.
+  Proof.
+    apply own_alloc_cofinite. done.
+  Qed.
 
   Lemma ghost_var_valid γ dq a :
     ghost_var γ dq a ⊢
     ⌜✓ dq⌝.
   Proof.
-    iIntros "H".
-    iDestruct (own_valid with "H") as %(? & _)%pair_valid.
-    iSteps.
+    rewrite /ghost_var own_valid dfrac_agree_validI //.
   Qed.
   Lemma ghost_var_combine γ dq1 a1 dq2 a2 :
     ghost_var γ dq1 a1 -∗
     ghost_var γ dq2 a2 -∗
-      ⌜a1 = a2⌝ ∗
+      a1 ≡ a2 ∗
       ghost_var γ (dq1 ⋅ dq2) a1.
   Proof.
-    iIntros "H1 H2". iCombine "H1 H2" as "H".
-    iDestruct (own_valid with "H") as %(? & ->)%dfrac_agree_op_valid_L.
-    rewrite -dfrac_agree_op. iSteps.
+    iIntros "H1 H2".
+    iCombine "H1 H2" as "H".
+    iDestruct (own_valid with "H") as "#Hvalid".
+    iDestruct (dfrac_agree_validI_2 with "Hvalid") as "(_ & Heq)".
+    iRewrite -"Heq" in "H".
+    rewrite -dfrac_agree_op. auto.
   Qed.
   Lemma ghost_var_valid_2 γ dq1 a1 dq2 a2 :
     ghost_var γ dq1 a1 -∗
     ghost_var γ dq2 a2 -∗
       ⌜✓ (dq1 ⋅ dq2)⌝ ∗
-      ⌜a1 = a2⌝.
+      a1 ≡ a2.
   Proof.
     iIntros "H1 H2".
-    iDestruct (ghost_var_combine with "H1 H2") as "(-> & H)".
-    iDestruct (ghost_var_valid with "H") as "$".
-    iSteps.
+    iDestruct (ghost_var_combine with "H1 H2") as "($ & H)".
+    iApply (ghost_var_valid with "H").
   Qed.
   Lemma ghost_var_agree γ dq1 a1 dq2 a2 :
     ghost_var γ dq1 a1 -∗
     ghost_var γ dq2 a2 -∗
-    ⌜a1 = a2⌝.
+    a1 ≡ a2.
   Proof.
     iIntros "H1 H2".
     iDestruct (ghost_var_valid_2 with "H1 H2") as "(_ & $)".
@@ -129,6 +148,71 @@ Section ghost_var_G.
   Proof.
     apply own_update, dfrac_agree_persist.
   Qed.
+  Section discrete.
+    Context `{!OfeDiscrete $ oFunctor_apply F $ iPropO Σ}.
+    Lemma ghost_var_combine_discrete γ dq1 a1 dq2 a2 :
+      ghost_var γ dq1 a1 -∗
+      ghost_var γ dq2 a2 -∗
+        ⌜a1 ≡ a2⌝ ∗
+        ghost_var γ (dq1 ⋅ dq2) a1.
+    Proof.
+      iIntros "H1 H2".
+      iDestruct (ghost_var_combine with "H1 H2") as "(% & $)".
+      iSteps.
+    Qed.
+    Lemma ghost_var_valid_2_discrete γ dq1 a1 dq2 a2 :
+      ghost_var γ dq1 a1 -∗
+      ghost_var γ dq2 a2 -∗
+        ⌜✓ (dq1 ⋅ dq2)⌝ ∗
+        ⌜a1 ≡ a2⌝.
+    Proof.
+      iIntros "H1 H2".
+      iDestruct (ghost_var_valid_2 with "H1 H2") as "($ & %)".
+      iSteps.
+    Qed.
+    Lemma ghost_var_agree_discrete γ dq1 a1 dq2 a2 :
+      ghost_var γ dq1 a1 -∗
+      ghost_var γ dq2 a2 -∗
+      ⌜a1 ≡ a2⌝.
+    Proof.
+      iIntros "H1 H2".
+      iDestruct (ghost_var_agree with "H1 H2") as %?.
+      iSteps.
+    Qed.
+    Section leibniz_equiv.
+      Context `{!LeibnizEquiv $ oFunctor_apply F $ iPropO Σ}.
+      Lemma ghost_var_combine_L γ dq1 a1 dq2 a2 :
+        ghost_var γ dq1 a1 -∗
+        ghost_var γ dq2 a2 -∗
+          ⌜a1 = a2⌝ ∗
+          ghost_var γ (dq1 ⋅ dq2) a1.
+      Proof.
+        iIntros "H1 H2".
+        iDestruct (ghost_var_combine_discrete with "H1 H2") as "(%Heq & $)".
+        apply leibniz_equiv in Heq.
+        iSteps.
+      Qed.
+      Lemma ghost_var_valid_2_L γ dq1 a1 dq2 a2 :
+        ghost_var γ dq1 a1 -∗
+        ghost_var γ dq2 a2 -∗
+          ⌜✓ (dq1 ⋅ dq2)⌝ ∗
+          ⌜a1 = a2⌝.
+      Proof.
+        iIntros "H1 H2".
+        iDestruct (ghost_var_valid_2_discrete with "H1 H2") as %(? & ?%leibniz_equiv).
+        iSteps.
+      Qed.
+      Lemma ghost_var_agree_L γ dq1 a1 dq2 a2 :
+        ghost_var γ dq1 a1 -∗
+        ghost_var γ dq2 a2 -∗
+        ⌜a1 = a2⌝.
+      Proof.
+        iIntros "H1 H2".
+        iDestruct (ghost_var_agree_discrete with "H1 H2") as %?%leibniz_equiv.
+        iSteps.
+      Qed.
+    End leibniz_equiv.
+  End discrete.
 
   Lemma ghost_var_update {γ a} a' :
     ghost_var γ (DfracOwn 1) a ⊢ |==>
